# 2485. Find the Pivot Integer
---

# Intuition

Iterate backwards from n

# Approach

- `if( pow(n,2) + n == 2*pow(x,2))`: It is a simplified version of
  `n*(n+1)/2 - x(x+1)/2 + x == x(x+1)/2`. As we need the sum of the intigers before and after `x` to be equal( **last `x` is due to the inclusive nature stated in the problem** ).
- `if( pow(n,2) + n > 2*pow(x,2))`: Onve the sum of the intigers before `x` become less thean the sum after `x`, there is no use in iterating more. So `return -1` directly.

# Complexity

- Time complexity: O(n)

- Space complexity: O(1)

# Code

```
class Solution {
public:
    int pivotInteger(int n) {

        if(n == 1)
            return 1;

        int x = n;
        while(x > 0) {
            if( pow(n,2) + n == 2*pow(x,2))
                return x;
            if( pow(n,2) + n > 2*pow(x,2))
                return -1;
            x--;
        }

        return -1;
    }
};
```
